Fix Conditions.toExpr
Signed-off-by: Zhengyao Lin <zyal@amazon.com>

cedar-lean/Cedar/Spec/Policy.lean
@@ -117,7 +117,7 @@ def Condition.toExpr (c : Condition) : Expr :=
 
 -- Conditions are evaluated top to bottom, and short circuit
 def Conditions.toExpr (cs : Conditions) : Expr :=
-  match cs with
+  match cs.reverse with
   | [] => Expr.lit (Prim.bool true)
   | c :: cs => cs.foldr (λ c expr => .and (c.toExpr) expr) c.toExpr
 
